src/Util/ListUtil/Forall.v
@@ -285,3 +285,65 @@ Lemma Forall2_trans {A B C} {AB BC} {xs : list A} {ys : list B} :
   Forall2 AB xs ys -> forall {zs : list C}, Forall2 BC ys zs ->
                                             Forall2 (fun x z => exists y, AB x y /\ BC y z) xs zs.
 Proof using Type. induction 1; inversion 1; subst; econstructor; eauto. Qed.
+
+Lemma Forall2_nil_nil_iff A B P
+  : @Forall2 A B P nil nil <-> True.
+Proof using Type. split; eauto. Qed.
+Lemma Forall2_nil_cons_iff A B P x y
+  : @Forall2 A B P nil (cons x y) <-> False.
+Proof using Type. split; firstorder inversion_one_head Forall2. Qed.
+Lemma Forall2_nil_l_iff A B P ls
+  : @Forall2 A B P nil ls <-> ls = nil.
+Proof using Type. split; firstorder (try inversion_one_head Forall2; subst; auto). Qed.
+Lemma Forall2_nil_r_iff A B P ls
+  : @Forall2 A B P ls nil <-> ls = nil.
+Proof using Type. split; firstorder (try inversion_one_head Forall2; subst; auto). Qed.
+Lemma Forall2_cons_nil_iff A B P x y
+  : @Forall2 A B P (cons x y) nil <-> False.
+Proof using Type. split; firstorder inversion_one_head Forall2. Qed.
+Lemma Forall2_cons_cons_iff A B P x xs y ys
+  : @Forall2 A B P (cons x xs) (cons y ys) <-> (P x y /\ Forall2 P xs ys).
+Proof using Type. split; firstorder (inversion_one_head Forall2; auto). Qed.
+Lemma Forall2_cons_l_ex_iff A B P x xs ls
+  : @Forall2 A B P (cons x xs) ls <-> (exists y ys, ls = cons y ys /\ P x y /\ Forall2 P xs ys).
+Proof using Type. split; firstorder (inversion_one_head Forall2; eauto). Qed.
+Lemma Forall2_cons_r_ex_iff A B P x xs ls
+  : @Forall2 A B P ls (cons x xs) <-> (exists y ys, ls = cons y ys /\ P y x /\ Forall2 P ys xs).
+Proof using Type. split; firstorder (inversion_one_head Forall2; eauto). Qed.
+
+Lemma pull_ex_Forall_iff {A B} {R : A -> B -> Prop} {ls}
+  : Forall (fun a => ex (R a)) ls <-> exists ls', Forall2 R ls ls'.
+Proof using Type.
+  induction ls as [|x xs IH];
+    rewrite ?Forall_nil_iff, ?Forall_cons_iff, ?IH;
+    try setoid_rewrite Forall2_nil_l_iff;
+    try setoid_rewrite Forall2_cons_l_ex_iff;
+    repeat firstorder (try inversion_one_head Forall; eauto 7).
+Qed.
+
+Lemma pull_ex_Forall2_l_iff {A B C} {R : A -> B -> C -> Prop} {ls1 ls2}
+  : Forall2 (fun a b => ex (R a b)) ls1 ls2 <-> exists ls3, List.length ls1 = List.length ls3 /\ Forall2 (fun ac b => R (fst ac) b (snd ac)) (List.combine ls1 ls3) ls2.
+Proof using Type.
+  revert ls2; induction ls1 as [|x xs IH], ls2 as [|y ys]; try specialize (IH ys).
+  all: rewrite ?Forall2_nil_nil_iff, ?Forall2_nil_cons_iff, ?Forall2_cons_nil_iff, ?Forall2_cons_cons_iff, ?IH.
+  all: try setoid_rewrite Forall2_nil_r_iff.
+  all: try setoid_rewrite Forall2_nil_l_iff.
+  all: try setoid_rewrite Forall2_cons_r_ex_iff.
+  all: repeat first [ progress cbn [List.length List.combine] in *
+                    | break_innermost_match_hyps_step
+                    | progress subst
+                    | solve [ exists nil; eauto ]
+                    | match goal with
+                      | [ H : S _ = S _ |- _ ] => inversion H; clear H
+                      | [ H : _ :: _ = _ :: _ |- _ ] => inversion H; clear H
+                      end
+                    | progress firstorder first [ congruence | eauto 7 ]
+                    | eexists (_ :: _) ].
+Qed.
+
+Lemma pull_ex_Forall2_r_iff {A B C} {R : A -> B -> C -> Prop} {ls1 ls2}
+  : Forall2 (fun a b => ex (R a b)) ls1 ls2 <-> exists ls3, List.length ls2 = List.length ls3 /\ Forall2 (fun a bc => R a (fst bc) (snd bc)) ls1 (List.combine ls2 ls3).
+Proof using Type.
+  setoid_rewrite Forall2_flip_iff; cbv [Basics.flip].
+  rewrite pull_ex_Forall2_l_iff; reflexivity.
+Qed.
